The bug vs dworkin is that he has the IV in the low bytes and the ctr in the high bytes but treats it little endian for addition; checkin before fix

src/crypto/aes/testctr.c
@@ -13,8 +13,6 @@
 */
 
 
-#define justfinalcall 1
-
 /* 
   Vale seems to be using the following calling conventions:
 
@@ -178,7 +176,6 @@ int test_make_ctr() {
   }
 }
 
-#ifndef justfinalcall
 void __stdcall CTR128Increment64StdCall(const void* input_ptr, void* output_ptr);
 
 int test_counter_increment_64() {
@@ -303,9 +300,6 @@ int test_counters_128() {
   }
 }
 
-#endif
-
-
 /* Key */
 const uint8_t k[]    = { 0x2b, 0x7e, 0x15, 0x16, 0x28, 0xae, 0xd2, 0xa6, 0xab, 0xf7, 0x15, 0x88, 0x09, 0xcf, 0x4f, 0x3c };
 /* Initial counter. */
@@ -329,7 +323,6 @@ const uint8_t output_block[][16] = {
 
 
 void __stdcall aes_main_i_KeyExpansionStdcall(const void * key_ptr, void *expanded_key_ptr);
-#ifndef justfinalcall
 void __stdcall AES128EncryptOneBlockStdcall(const void *output, const void *input, const void *expanded_key);
 
 int test_key_aes_encryption() {
@@ -359,9 +352,12 @@ int test_key_aes_encryption() {
   }
   return status;
 }
-#endif
 
 /*
+ What Dworkin must mean here for input block is the CTR going into AES at that key. 
+Output block is that CTR  being encrypted. It is then XORd with the plain text
+to get the cypher text.
+
 F.5.1       CTR-AES128.Encrypt       
 Key            2b7e151628aed2a6abf7158809cf4f3c      
 Init. Counter  f0f1f2f3f4f5f6f7f8f9fafbfcfdfeff  
@@ -398,7 +394,6 @@ const uint8_t C[][16]    = { { 0x87, 0x4d, 0x61, 0x91, 0xb6, 0x20, 0xe3, 0x26, 0
                              { 0x5a, 0xe4, 0xdf, 0x3e, 0xdb, 0xd5, 0xd3, 0x5e, 0x5b, 0x4f, 0x09, 0x02, 0x0d, 0xb0, 0x3e, 0xab},
                              { 0x1e, 0x03, 0x1d, 0xda, 0x2f, 0xbe, 0x03, 0xd1, 0x79, 0x21, 0x70, 0xa0, 0xf3, 0x00, 0x9c, 0xee}};
 
-#ifndef justfinalcall
 // The standard calling sequence of x86 on both windows/linux will give us four arguments in registers.
 
 void __stdcall CTREncryptOneBlockStdCall(const void* expanded_key, const void* counter, const void* input_ptr, void* output_ptr);
@@ -408,12 +403,20 @@ int test_encryption_one_block() {
   int status = 1;
   uint8_t expanded_key[176];
   aes_main_i_KeyExpansionStdcall(k, expanded_key);
-  for (int i = 0; i < 4; ++i) {
+  for (int i = 0; i < 1; ++i) {
     uint8_t *output = malloc(sizeof(uint8_t) * 16);
-    // Actually passing args in rax, esi, rsi and rdx.
+    // WTF? I'm not passing in the counter and this works? ==> ctr is zero?
+    // rsi is hanging around from the key expansion, but it works. Why?
     CTREncryptOneBlockStdCall(expanded_key, input_block+i, P+i, output);
-    if (memcmp(output, C+i, sizeof(uint8_t) *16) == 0) {
-      printf("AES128 Encrypt One Block CTR P[%d] succeded.\n",i);
+    if (memcmp(output, C+i, sizeof(uint8_t) * 16) == 0) {
+      printf("AES128 Encrypt One Block CTR P[%d] succeded.\n\n",i);
+      // Temporary printing.
+  	printf("AES128 Encrypt One Block CTR P[%d] \n",i );
+  	print128BitVectorHex((uint8_t *)P+i);
+  	printf("AES128 Encrypt One Block CTR C[%d] \n",i);
+  	print128BitVectorHex((uint8_t *)C+i);
+  	printf("AES128 Encrypt One Block CTR output \n");
+  	print128BitVectorHex(output);
     } else {
       printf("AES128 Encrypt One Block CTR P[%d] failed.\n", i);
       if (trace == 1) {
@@ -456,7 +459,6 @@ int test_decryption_one_block() {
   }
   return status;
 }
-#endif
 
 /* Plain text. */
 const uint8_t PStream[64]    = {  0x6b, 0xc1, 0xbe, 0xe2, 0x2e, 0x40, 0x9f, 0x96, 0xe9, 0x3d, 0x7e, 0x11, 0x73, 0x93, 0x17, 0x2a,
@@ -500,17 +502,28 @@ int test_encrypt_stream() {
   aes_main_i_KeyExpansionStdcall(k, expanded_key);
 
   uint8_t *CypherText = (uint8_t *)malloc(sizeof(uint8_t) * 64); 
-  uint64_t iv = 0xf0f1f2f3f4f5f6f7;
+  // 4 ways
+  // iv = 0xf0f1f2f3f4f5f6f7; init_ctr = 0xf8f9fafbfcfdfeff; - no 
+  // iv = 0xf8f9fafbfcfdfeff; init_ctr = 0xf0f1f2f3f4f5f6f7; - no 
+  // iv = 0xfffefdfcfbfaf9f8; init_ctr = 0xf7f6f5f4f3f2f1f0; - yes, first block succeeds second does not.
+  // So he has the IV in the low bytes, reversed and the ctr in the high bytes and is treating it
+  // little endian.
+  uint64_t iv = 0xfffefdfcfbfaf9f8;
   // Damn it, Dworkin did not start the counter at ZERO in the text code.
-  uint64_t init_ctr = 0xf8f9fafbfcfdfeff;
+  uint64_t init_ctr = 0xf7f6f5f4f3f2f1f0;
 
   // In CTR mode one just encrypts a ctr with a key in sequence and
   // XORs it with the input. So the decrypt is to just run it in the
   // other direction.
-  CTR128EncryptStdcall(k, (const void*)((size_t)PStream + sizeof(PStream)), (const void *)iv, 
-                       PStream, expanded_key, CypherText, (const void*)init_ctr);
+  CTR128EncryptStdcall(k,                                                       //edi
+                       (const void*)((size_t)PStream + 32 /*sizeof(PStream)*/), //esi
+                       (const void *)iv,                                        //rdx
+                       PStream,                                                 //rcx
+                       expanded_key,                                            //r8
+                       CypherText,                                              //r9
+                       (const void*)init_ctr);                                  //stack
 
-  if (memcmp(CypherText,CStream,64) == 0) {
+  if (memcmp(CypherText,CStream,32) == 0) {
     printf("AES128 CTR Encrypt Stream success\n");
   } else {
     printf("AES128 CTR Encrypt Stream failure\n");
@@ -526,39 +539,8 @@ int test_encrypt_stream() {
   return status;
 }
 
-#ifndef justfinalcall
-
 int test_decrypt_stream() {
-  printf("\nTest AES Decrypt Stream \n");
-  int status = 1;
-
-  uint8_t expanded_key[176];
-  aes_main_i_KeyExpansionStdcall(k, expanded_key);
-
-  uint8_t CypherText[64]; 
-  // Damn it, Dworkin did not start the counter at ZERO.
-  uint64_t iv = 0xf0f1f2f3f4f5f60xf7;
-
-  // In CTR mode one just encrypts a ctr with a key in sequence and
-  // XORs it with the input. So the decrypt is to just run it in the
-  // other direction.
-  CTR128EncryptStdcall(k, (const void*)((size_t)CStream + sizeof(CStream)), (const void *)iv, 
-                       CStream, expanded_key, CypherText, (const void*)init_ctr);
-  // Why scratch?
-  if (memcmp(CypherText,PStream,64) == 0) {
-    printf("AES128 CTR Decrypt Stream success\n");
-  } else {
-    printf("AES128 CTR Decrypt Stream failure\n");
-    printf("AES128 CTR Decrypt Stream Input  stream\n");
-    print_stream(PStream);
-    printf("AES128 CTR Decrypt Stream Output stream\n");
-    print_stream(CypherText);
-    printf("AES128 CTR Decrypt Stream Should Be stream\n");
-    print_stream(CStream);
-    return 0;
-  }
-
-  return status;
+  return 1;
 }
 
 int test_encryption() {
@@ -576,17 +558,16 @@ int test_decryption() {
   return (b1 == 1) && (stream == 1);
 }
 
-
 int __cdecl main(void) {
   //  test_alignment_in_memory();
-  test_make_ctr();
-  int tc64 = test_counters_64();
-  int tc128 = test_counters_128();
-  int tk = test_key_aes_encryption();
-  int te = test_encryption();
-  int td = test_decryption();
-  
-  int status = (tk == 1 && tc64 == 1 && tc128 == 1 && te == 1 && td == 1);
+  //test_make_ctr();
+  //  int tc64 = test_counters_64();
+  //  int tc128 = test_counters_128();
+  //  int tk = test_key_aes_encryption();
+    int te = test_encryption();
+  //  int td = test_decryption();
+  //int status = (tk == 1 && tc64 == 1 && tc128 == 1 && te == 1 && td == 1);
+  int status = 0;
 
   if (status == 1) {
     printf("AES128 CTR all tests succeded.\n");
@@ -597,11 +578,5 @@ int __cdecl main(void) {
   }
 }
 
-#endif
 
-#ifdef justfinalcall
-int __cdecl main(void) {
-  //  test_alignment_in_memory();
-  test_encrypt_stream();
-}
-#endif
+
