src/crypto/aes/aes-x64/ctr_helpers.i.dfy
@@ -1,19 +1,316 @@
+include "../../../lib/util/types.s.dfy"
+include "../../../lib/util/operations.s.dfy"
+include "../../../lib/util/words_and_bytes.s.dfy"
+include "../../../lib/collections/Seqs.s.dfy"
 include "../../../arch/x64/vale.i.dfy"
 include "../../../lib/util/dafny_wrappers.i.dfy"
-include "../cbc.s.dfy"
-include "../aes.s.dfy"
-include "../aes_helpers.i.dfy"
 
 include "../ctr.s.dfy"
 
-module CTR_Helpers {
-import opened x64vale_CTR_temp = x64_vale_i
-import opened parser_help_i_CTR_temp = dafny_wrappers_i 
-import opened CBCModule_CTR_helpers_tmp = CBCModule
-import opened AESModule_CTR_helpers_tmp = AESModule
-import opened AESHelpersModule_CTR_helpers_tmp = AESHelpersModule
+include "../aes.s.dfy"
+include "../aes_helpers.i.dfy"
 
+module CTRHelpers {
+
+import opened x64_vale_i
+import opened x64_def_s
+import opened types_s
+import opened dafny_wrappers_i
+import opened AESModule
+import opened AESHelpersModule
 import opened CTRModule
 
+// Use a ghost var of G, for ghosts, to cut the size of the code.
+datatype G = G(ghost key : seq<uint32>,
+               ghost key_heap : heaplet_id,
+               ghost exp_key : seq<uint32>,
+               ghost exp_key_heap : heaplet_id,
+               ghost inp :seq<Quadword>,
+               ghost inp_heap : heaplet_id,
+               ghost out_heap : heaplet_id,
+               ghost alg: Algorithm)
 
+
+// Bind the registers, passed as operators, to a physical register.
+predicate BindRegsPhy1(key_ptr : operand, exp_key_ptr : operand, iv_reg : operand, inp_ptr : operand, inp_end_ptr : operand,  out_ptr : operand, ctr_reg : operand, init_ctr : operand) {
+ key_ptr.OReg?      && key_ptr     == OReg(X86Edi) &&
+ exp_key_ptr.OReg?  && exp_key_ptr == OReg(X86R8) && 
+ iv_reg.OReg?       && iv_reg      == OReg(X86Edx) && 
+ inp_ptr.OReg?      && inp_ptr     == OReg(X86Ecx) && 
+ inp_end_ptr.OReg?  && inp_end_ptr == OReg(X86Esi) &&
+ out_ptr.OReg?      && out_ptr     == OReg(X86R9) &&
+ ctr_reg.OReg?      && ctr_reg     == OReg(X86Xmm(4)) &&
+ init_ctr.OReg?     && init_ctr    == OReg(X86R12) 
+}
+
+predicate BindRegsPhy1Curr(key_ptr : operand, exp_key_ptr : operand, iv_reg : operand, 
+                           inp_ptr : operand, inp_end_ptr : operand,  
+                           out_ptr : operand, ctr_reg : operand,
+                           init_ctr : operand,
+                           curr_inp_ptr : operand, curr_out_ptr : operand) {
+  BindRegsPhy1(key_ptr, exp_key_ptr, iv_reg, inp_ptr, inp_end_ptr, out_ptr, ctr_reg, init_ctr) && 
+  curr_inp_ptr.OReg? && curr_inp_ptr  == OReg(X86R10) &&   
+  curr_out_ptr.OReg? && curr_out_ptr == OReg(X86R11)
+}
+
+// Memory
+predicate Mem128ChangedOnlyIn(regptr : uint64, count : int, heap : heaplet_id, mem : Heaplets, oldmem: Heaplets)
+{
+    heap in mem &&
+    mem == oldmem[heap := mem[heap]] &&
+    mem[heap].QuadwordHeaplet? &&
+    heap in oldmem &&
+    oldmem[heap].QuadwordHeaplet? &&
+    forall a :: (a < regptr || a >= regptr + count * 16) &&
+     a in mem[heap].quads ==> a in oldmem[heap].quads &&
+     mem[heap].quads[a] == oldmem[heap].quads[a]
+}
+
+predicate Mem64ChangedOnlyIn(regptr : uint64, count : int, heap : heaplet_id, mem : Heaplets, oldmem: Heaplets)
+{
+    heap in mem &&
+    mem == oldmem[heap := mem[heap]] &&
+    mem[heap].Heaplet64? &&
+    heap in oldmem &&
+    oldmem[heap].Heaplet64? &&
+    forall a :: (a < regptr || a >= regptr + count * 8) &&
+     a in mem[heap].mem64 ==> a in oldmem[heap].mem64 &&
+     mem[heap].mem64[a] == oldmem[heap].mem64[a]
+}
+
+predicate QuadwordSeqInMemory(qws : seq<Quadword>, mem: Heaplet, ptr : uint64) 
+  requires mem.QuadwordHeaplet?
+{
+    forall b:int :: 0 <= b < |qws| ==> ptr + b*16 in mem.quads && mem.quads[ptr + b*16].v == qws[b]  
+}
+
+// TODO obviate 
+predicate CtrInMem(ctr : Quadword, regptr : uint64, heap : heaplet_id, mem : Heaplets) { 
+  // That register's value points to a readable source addresss in that heap with public taint.
+  ValidSrcAddr(mem, heap, regptr, 128, Public) &&
+  mem[heap].QuadwordHeaplet? &&
+  ctr == mem[heap].quads[regptr].v
+}
+
+lemma lemma_BitwiseAdd64()
+    ensures  forall x:uint64, y:uint64 :: x + y < 0x1_0000_0000_0000_0000 ==> BitwiseAdd64(x, y) == x + y
+    ensures  forall x:uint64, y:uint64 :: x + y >= 0x1_0000_0000_0000_0000 ==> BitwiseAdd64(x, y) == x + y - 0x1_0000_0000_0000_0000
+    ensures  forall x:uint64 :: BitwiseAdd64(x, 0) == x;
+{
+    reveal_BitwiseAdd64();
+}
+
+predicate CtrIncr(oldc : Quadword, newc : Quadword) {
+  oldc.hi     == newc.hi &&
+  oldc.mid_hi == newc.mid_hi &&
+  newc.mid_lo == upper64(BitwiseAdd64(lowerUpper64(oldc.lo,oldc.mid_lo), 1)) &&
+  newc.lo     == lower64(BitwiseAdd64(lowerUpper64(oldc.lo,oldc.mid_lo), 1))
+}
+
+predicate CtrIncrN(newc : Quadword, init_ctr : uint64, n : nat) 
+ requires n < 1_0000_0000_0000_0000;
+{
+// I'm the init_ctr + n with wrapping.
+  newc.mid_lo == upper64(BitwiseAdd64(init_ctr, n)) &&
+  newc.lo     == lower64(BitwiseAdd64(init_ctr, n))
+}
+
+lemma lemma_CtrIncrNTrans(old_ctr : Quadword, new_ctr: Quadword, init_ctr : uint64, n : nat)
+  requires n + 1 < 1_0000_0000_0000_0000;
+  requires CtrIncrN(old_ctr, init_ctr, n);
+  requires CtrIncr (old_ctr,  new_ctr);
+  ensures  CtrIncrN(new_ctr, init_ctr, n + 1);
+{
+  lemma_BitwiseAdd64();
+  reveal_BitwiseAdd64();
+  reveal_upper64();
+  reveal_lower64();
+  reveal_lowerUpper64();
+}
+
+predicate AlgReq(g : G, key_ptr : uint64) {
+  g.alg == AES_128 &&
+  |g.key| == Nk(g.alg) && 
+  SeqLength(g.key) == Nk(g.alg) &&
+  (Nb() * (Nr(g.alg) + 1)) / 4 == Nr(g.alg) + 1 &&   // Easy to prove, but necessary precondition to Cipher
+  (Nb() * (Nr(g.alg) + 1)) % 4 == 0 &&   // Easy to prove, but necessary precondition to Cipher
+  key_ptr % 16 == 0
+}
+
+predicate HeapReq(g : G, mem : Heaplets, old_mem : Heaplets) {
+// In the memory
+  g.key_heap in mem &&  g.exp_key_heap in mem &&  g.inp_heap in mem &&  g.out_heap in mem &&
+  g.key_heap in old_mem &&  g.exp_key_heap in old_mem &&  g.inp_heap in old_mem &&  g.out_heap in old_mem &&
+
+// Disjointness.
+  g.key_heap != g.exp_key_heap &&
+  g.key_heap != g.inp_heap &&
+  g.key_heap != g.out_heap &&
+  g.exp_key_heap != g.inp_heap &&
+  g.exp_key_heap != g.out_heap &&
+  g.inp_heap != g.out_heap &&
+
+// Types of heaplets in memory.
+  mem[g.inp_heap].QuadwordHeaplet? &&
+  mem[g.out_heap].QuadwordHeaplet? &&
+
+// Heaplets don't change.
+  mem[g.key_heap]    == old_mem[g.key_heap] &&
+  mem[g.exp_key_heap] == old_mem[g.exp_key_heap] &&
+  mem[g.inp_heap] == old_mem[g.inp_heap]
+}
+
+predicate KeyReq(g : G, exp_key_ptr : uint64, mem : Heaplets) {
+  ValidSrcAddrs(mem, g.exp_key_heap, exp_key_ptr, 128, Secret, 11*16) &&   // Key is readable
+  exp_key_ptr % 16 == 0 &&
+  SeqLength(g.exp_key) == 44 
+}
+
+predicate ExpKeyReq(g : G, key_ptr : uint64, exp_key_ptr : uint64, mem : Heaplets) {
+  AlgReq(g, key_ptr) &&
+  KeyReq(g, exp_key_ptr, mem) &&
+  (forall j :: 0 <= j <= 10 ==> mem[g.exp_key_heap].quads[exp_key_ptr + 16*j].v == 
+         Quadword(g.exp_key[4*j], g.exp_key[4*j+1], g.exp_key[4*j+2], g.exp_key[4*j+3])) &&
+    KeyExpansionPredicate(g.key, g.alg, g.exp_key)
+}
+
+predicate InpInMem(g : G, inp_ptr : uint64, inp_end_ptr : uint64, mem : Heaplets) {
+  // TODO - 1 weakens the length of sequence.
+  0 < SeqLength(g.inp) < 1_0000_0000_0000_0000 - 1 &&
+  ValidSrcAddrs(mem, g.inp_heap, inp_ptr, 128, Secret, SeqLength(g.inp)*16) &&
+  QuadwordSeqInMemory(g.inp, mem[g.inp_heap], inp_ptr)
+}
+
+predicate OutWriteable(inp : seq<Quadword>, out_heap : heaplet_id, 
+                       out_ptr : uint64, mem : Heaplets) {
+  ValidSrcAddrs(mem, out_heap, out_ptr, 128, Secret, SeqLength(inp)*16)
+}
+
+predicate InpOutInvariants(inp : seq<Quadword>, inp_ptr : uint64, inp_end_ptr : uint64, 
+                               out_ptr : uint64) {
+   inp_ptr + SeqLength(inp)*16 < 0x1_0000_0000_0000_0000 &&
+   out_ptr + SeqLength(inp)*16 < 0x1_0000_0000_0000_0000 &&
+   inp_end_ptr >= inp_ptr && 
+   inp_end_ptr == inp_ptr + SeqLength(inp)*16 &&
+   inp_end_ptr < 0x1_0000_0000_0000_0000 
+}
+
+// On the call, what is true before the setup?
+predicate CTRInvInit(g : G,
+    key_ptr : uint64, exp_key_ptr : uint64,
+    inp_ptr : uint64, inp_end_ptr : uint64,
+    out_ptr : uint64,
+    iv_reg  : uint64,
+    mem : Heaplets, 
+    old_mem : Heaplets)
+{
+        HeapReq(g, mem, old_mem) &&
+        KeyReq(g, key_ptr, mem) &&
+        ExpKeyReq(g, key_ptr, exp_key_ptr, mem) &&
+        InpInMem(g, inp_ptr, inp_end_ptr, mem) &&
+        OutWriteable(g.inp, g.out_heap, out_ptr, mem) &&
+        InpOutInvariants(g.inp, inp_ptr, inp_end_ptr, out_ptr) &&
+        mem == old_mem[g.out_heap := mem[g.out_heap]]
+}
+
+predicate CTRInv(g : G,
+    key_ptr : uint64, exp_key_ptr : uint64,
+    inp_ptr : uint64, inp_end_ptr : uint64,
+    out_ptr : uint64,
+    iv_reg  : uint64,
+    ctr_reg : Quadword,
+    mem : Heaplets, 
+    old_mem : Heaplets)
+{
+   CTRInvInit(g, key_ptr, exp_key_ptr, inp_ptr, inp_end_ptr, out_ptr, iv_reg, mem, old_mem)
+}
+
+predicate CtrInvBefore(iv_reg : uint64, ctr_reg : Quadword, init_ctr : uint64, blocktobecopied : nat) {
+  blocktobecopied + 1 < 1_0000_0000_0000_0000 &&
+  ctr_reg == ctr_n(iv_reg, init_ctr, blocktobecopied) &&
+  ctr_reg.hi == upper64(iv_reg) &&
+  ctr_reg.mid_hi == lower64(iv_reg) &&
+  ctr_reg.mid_lo == upper64(BitwiseAdd64(init_ctr, blocktobecopied)) &&
+  ctr_reg.lo     == lower64(BitwiseAdd64(init_ctr, blocktobecopied))
+}
+
+predicate CtrInvAfter(iv_reg : uint64, ctr_reg : Quadword, init_ctr : uint64, blocktobecopied : nat) 
+{
+  reveal_BitwiseAdd64();
+  reveal_upper64();
+  reveal_lower64();
+  reveal_lowerUpper64();
+
+  blocktobecopied < 1_0000_0000_0000_0000 &&
+  ctr_reg == ctr_n(iv_reg, init_ctr, blocktobecopied) &&
+  ctr_reg.hi == upper64(iv_reg) &&
+  ctr_reg.mid_hi == lower64(iv_reg) &&
+  ctr_reg.mid_lo == upper64(BitwiseAdd64(init_ctr, blocktobecopied)) &&
+  ctr_reg.lo     == lower64(BitwiseAdd64(init_ctr, blocktobecopied))
+}
+
+predicate CopyInvAlways(g : G,
+                  inp_ptr : uint64, inp_end_ptr : uint64, curr_inp_ptr : uint64,
+                  out_ptr : uint64, curr_out_ptr : uint64,
+                  blockscopied : int) {
+     curr_inp_ptr == inp_ptr + blockscopied * 16 &&
+     curr_out_ptr == out_ptr + blockscopied * 16 &&
+     inp_end_ptr  == inp_ptr  + SeqLength(g.inp) * 16
+}
+
+predicate InputInOutputMem(g : G, out_ptr : uint64, iv_reg : uint64, init_ctr : uint64, ctr_reg : Quadword, key_ptr : uint64,
+                           mem : Heaplets, blockscopied : int)
+ requires |g.inp| < 1_0000_0000_0000_0000;
+ requires g.out_heap in mem;
+ requires ValidSrcAddrs(mem, g.out_heap, out_ptr, 128, Secret, |g.inp|* 16)
+ requires AlgReq(g, key_ptr);
+{
+  0 <= blockscopied <= |g.inp| &&
+  forall j: nat :: 0 <= j < blockscopied ==>
+  // Three steps in developing this predicate.
+  // 1) just copy.
+  // inp[j] == mem[g.out_heap].quads[out_ptr + j * 16].v 
+  // 2) copy the ctr xor'd with the data.
+  // QuadwordXor(inp[j], ctr_n(iv_reg, init_ctr, j)) == mem[g.out_heap].quads[out_ptr + j * 16].v
+  // 3) copy the ctr encrypted xor'd with the data == AES-CTR.
+  QuadwordXor(g.inp[j], AES_Encrypt(g.key, ctr_n(iv_reg, init_ctr, j), g.alg))
+           == mem[g.out_heap].quads[out_ptr + j * 16].v
+}
+
+predicate CopyInvBefore(g : G,
+                       inp_ptr : uint64, inp_end_ptr : uint64, curr_inp_ptr : uint64,
+                       out_ptr : uint64, curr_out_ptr : uint64,
+                       iv_reg : uint64, init_ctr : uint64, ctr_reg : Quadword, key_ptr : uint64,
+                       mem : Heaplets,
+                       blocktobecopied : int) 
+ requires |g.inp| < 1_0000_0000_0000_0000;
+ requires g.out_heap in mem;
+ requires ValidSrcAddrs(mem, g.out_heap, out_ptr, 128, Secret, |g.inp|* 16);
+ requires AlgReq(g, key_ptr);
+{
+     CopyInvAlways(g, inp_ptr, inp_end_ptr, curr_inp_ptr, out_ptr, curr_out_ptr, blocktobecopied) &&
+     inp_ptr <= curr_inp_ptr <= inp_end_ptr &&
+     0 <= blocktobecopied < |g.inp| &&
+     InputInOutputMem(g, out_ptr, iv_reg, init_ctr, ctr_reg, key_ptr, mem, blocktobecopied)
+}
+
+predicate CopyInvAfter(g : G,
+                       inp_ptr : uint64, inp_end_ptr : uint64, curr_inp_ptr : uint64,
+                       out_ptr : uint64, curr_out_ptr : uint64, 
+                       iv_reg : uint64, init_ctr : uint64, ctr_reg : Quadword, key_ptr : uint64,
+                       mem : Heaplets, old_mem : Heaplets,
+                       blockscopied : int)
+  requires |g.inp| < 1_0000_0000_0000_0000;
+  requires 0 <= blockscopied <= |g.inp|;
+  requires g.out_heap in mem;
+  requires mem[g.out_heap].QuadwordHeaplet?;
+  requires ValidSrcAddrs(mem, g.out_heap, out_ptr, 128, Secret, |g.inp|* 16)
+  requires AlgReq(g, key_ptr);
+{
+     CopyInvAlways(g, inp_ptr, inp_end_ptr, curr_inp_ptr, out_ptr, curr_out_ptr, blockscopied) &&
+     inp_ptr <= curr_inp_ptr <= inp_end_ptr &&
+     InputInOutputMem(g, out_ptr, iv_reg, init_ctr, ctr_reg, key_ptr, mem, blockscopied)
+}
+
+// End of Module
 }
