src/crypto/aes/ctr.s.dfy
@@ -2,35 +2,54 @@ include "../../lib/util/types.s.dfy"
 include "../../lib/util/operations.s.dfy"
 include "../../lib/util/words_and_bytes.s.dfy"
 include "../../lib/collections/Seqs.s.dfy"
+include "../../arch/x64/def.s.dfy"
 include "aes.s.dfy"
 
 module CTRModule {
 
+import opened x64_def_s
 import opened types_s
 import opened AESModule
 
-//function CTR_Encrypt_One_Block(key:seq<uint32>, input:Quadword, alg:Algorithm, counter:Quadword) : Quadword
-//    requires |key| == Nk(alg);
-//    requires (Nb() * (Nr(alg) + 1)) / 4 == Nr(alg) + 1;   // Easy to prove, but necessary precondition to Cipher
-//    requires (Nb() * (Nr(alg) + 1)) % 4 == 0;   // Easy to prove, but necessary precondition to Cipher
-//{
-//      QuadwordXor(input, AES_Encrypt(key, counter, alg))
-//}
-//
-//function CTR_EncryptTODO(key:seq<uint32>, input:seq<Quadword>, alg:Algorithm, counter:Quadword) : seq<Quadword>
-//    requires |key| == Nk(alg);
-//    requires |input| > 0;
-//    requires |input| < 0x1_0000_0000_0000_0000;
-//    requires (Nb() * (Nr(alg) + 1)) / 4 == Nr(alg) + 1;   // Easy to prove, but necessary precondition to Cipher
-//    requires (Nb() * (Nr(alg) + 1)) % 4 == 0;   // Easy to prove, but necessary precondition to Cipher
-//{
-//    if |input| == 1 then
-//      [QuadwordXor(input[0], AES_Encrypt(key, counter, alg))]
-//    else
-//      var first := [QuadwordXor(input[0], AES_Encrypt(key, counter, alg))];
-//      var next_counter := CTR_increment_counter(counter);
-//      first + CTR_Encrypt(key, all_but_first(input), alg, next_counter)
-//}
+// The counter at N increments.
+function ctr_n(iv : uint64, init_ctr : uint64, n : uint64) : Quadword 
+{
+  reveal_BitwiseAdd64();
+  reveal_upper64();
+  reveal_lower64();
+  Quadword(lower64(BitwiseAdd64(init_ctr,n)), 
+           upper64(BitwiseAdd64(init_ctr,n)),
+           lower64(iv), 
+           upper64(iv))
+}
+
+
+predicate CTR_EncryptReq(key:seq<uint32>, input:seq<Quadword>, alg:Algorithm, n : uint64) {
+    |input| > 0 &&
+    |input| < 0x1_0000_0000_0000_0000 - 1 &&
+    n + |input| < 0x1_0000_0000_0000_0000 - 1 &&
+    |key| == Nk(alg) &&
+    (Nb() * (Nr(alg) + 1)) / 4 == Nr(alg) + 1 &&
+    (Nb() * (Nr(alg) + 1)) % 4 == 0
+}
+
+function CTR_EncryptAt(key:seq<uint32>, input:seq<Quadword>, alg:Algorithm, iv : uint64, init_ctr : uint64, n : uint64) : Quadword
+    requires CTR_EncryptReq(key, input, alg, n);
+    decreases |input|;
+{
+     QuadwordXor(input[0], AES_Encrypt(key, ctr_n(iv, init_ctr, n), alg))
+}
+
+function CTR_Encrypt(key:seq<uint32>, input:seq<Quadword>, alg:Algorithm, iv : uint64, init_ctr : uint64, n : uint64) : seq<Quadword>
+    decreases |input|;
+    requires CTR_EncryptReq(key, input, alg, n);
+{
+    if |input| == 1 then
+      [QuadwordXor(input[0], AES_Encrypt(key, ctr_n(iv, init_ctr, n), alg))]
+    else
+      var first := [CTR_EncryptAt(key,input,alg, iv, init_ctr, n)];
+      first + CTR_Encrypt(key, all_but_first(input), alg, iv, init_ctr, n + 1)
+}
 
 // We don't need a decrypt predicate as the standard uses encrypt again and the xor decrypts.
 }
