SConscript
@@ -34,6 +34,8 @@ verify_options = {
   'obj/crypto/aes/cbc.gen.dfy': BuildOptions(dafny_default_args_nonlarith + ' /timeLimit:120'),
   'obj/crypto/aes/aes-x64/cbc.gen.dfy': BuildOptions(dafny_default_args_nonlarith + ' /timeLimit:120'),
 
+  'obj/crypto/aes/aes-x64/ctr.gen.dfy': BuildOptions(dafny_default_args_nonlarith + ' /timeLimit:120' + ' /noVerify'),
+
   # .dfy files default to this set of options
   '.dfy': BuildOptions(dafny_default_args_nonlarith),
 
